KeyManagement/Simulation.v
@@ -51,14 +51,14 @@ Inductive action_matches : forall {A B : Type},
                            RealWorld.action -> RealWorld.universe A B ->
                            IdealWorld.action -> IdealWorld.universe A -> Prop :=
 | Inp : forall A B t__r t__i (m__rw : RealWorld.crypto t__r) (m__iw m__expected : IdealWorld.message.message t__i)
-               ms (U__rw : RealWorld.universe A B) (U__iw : IdealWorld.universe A) rw iw ch_id cs ps p,
-      rw = (RealWorld.Input m__rw p)
+               ms (U__rw : RealWorld.universe A B) (U__iw : IdealWorld.universe A) rw iw ch_id cs ps p froms,
+      rw = (RealWorld.Input m__rw p froms)
       -> iw = IdealWorld.Input m__iw ch_id cs ps
       -> U__iw.(IdealWorld.channel_vector) $? ch_id = Some ((existT _ _ m__expected) :: ms)
       -> MessageEq.message_eq m__rw U__rw m__iw U__iw m__expected ch_id {} {}
       -> action_matches rw U__rw iw U__iw
-| Out : forall A B t__r t__i (m__rw : RealWorld.crypto t__r) (m__iw m__expected : IdealWorld.message.message t__i) ms (U__rw : RealWorld.universe A B) (U__iw : IdealWorld.universe A) rw iw ch_id cs ps suid,
-    rw = RealWorld.Output m__rw suid
+| Out : forall A B t__r t__i (m__rw : RealWorld.crypto t__r) (m__iw m__expected : IdealWorld.message.message t__i) ms (U__rw : RealWorld.universe A B) (U__iw : IdealWorld.universe A) rw iw ch_id cs ps suid to_q to_froms,
+    rw = RealWorld.Output m__rw suid to_q to_froms
     -> iw = IdealWorld.Output m__iw ch_id cs ps
     -> U__iw.(IdealWorld.channel_vector) $? ch_id = Some (ms ++ [existT _ _ m__expected])
     -> MessageEq.message_eq m__rw U__rw m__iw U__iw m__expected ch_id {} {}
